Circuit/CircuitBase.dfy
@@ -1,0 +1,208 @@
+module CircuitBase {
+
+    import opened Std.Wrappers
+    import Std.Collections.Seq
+
+    newtype CPort = nat
+    const INPUT_PORT: CPort := 0
+    const OUTPUT_PORT: CPort := 1
+
+    // A node in the graph.
+    newtype CNode = nat
+
+    datatype NP = NP(n: CNode, p: CPort)
+
+    // HPINP and HPONP can reference a port nested in the hierarchy.
+    // This is useful as an intermediate when converting to a HGraph.
+
+    datatype HPNP = HPNP(hpn: HPNode, p: CPort)
+
+    // Represents the path taken through a hierarchy of nodes where a node can
+    // represent a lower-level circuit.
+    datatype HierarchyPath = HP(v: seq<CNode>)
+
+    datatype HPNode =
+        HPNode(
+            hp: HierarchyPath,
+            n: CNode
+        )
+
+    datatype Circuit = Circuit(
+        NodeKind: CNode -> Option<CNodeKind>,
+        PortSource: NP -> Option<NP>,
+        // This is larger or equal to all nodes for which NodeKind(node) is Some
+        // We use this help dafny prove that things are finite and terminate.
+        NodeBound: CNode,
+        PortBound: CPort,
+        HierLevel: nat,
+        PortNames: string -> Option<CNode>
+    )
+
+    datatype CNodeKind = 
+        // A hierarchical node so we can design hierarchically.
+      | CHier(c: Circuit)
+        // A node representing combinatorial logic.
+      | CComb(
+          IPorts: seq<CPort>,
+          OPorts: seq<CPort>,
+          PathExists: (CPort, CPort) -> bool,
+          Behav: map<CPort, bool> -> Option<map<CPort, bool>>,
+          PortNames: string -> Option<CPort>
+        )
+        // A contant 0 or 1
+      | CConst(value: bool)
+        // An input to the circuit.
+      | CInput()
+        // An output from the circuit.
+      | COutput()
+        // A register.
+      | CSeq()
+
+    function IPorts(nk: CNodeKind): set<CPort>
+    {
+        match nk
+        // The port numbers of a hierarical block and just the node ids of
+        // the input and output nodes.
+        case CHier(subc) =>
+            set n | n < subc.NodeBound && subc.NodeKind(n) == Some(CInput) :: n as CPort
+        case CComb(iports, oports, path_exists, behav, names) => Seq.ToSet(iports)
+        case CInput() => {}
+        case CConst(v) => {}
+        case COutput() => {0 as CPort}
+        case CSeq() => {0 as CPort}
+    }
+
+    predicate IsIPort(nk: CNodeKind, p: CPort)
+    {
+        match nk
+        // The port numbers of a hierarical block and just the node ids of
+        // the input and output nodes.
+        case CHier(subc) => subc.NodeKind(p as CNode) == Some(CInput)
+        case CComb(iports, oports, path_exists, behav, name) => p in iports
+        case CInput() => false
+        case CConst(v) => false
+        case COutput() => p == INPUT_PORT as CPort
+        case CSeq() => p == INPUT_PORT as CPort
+    }
+
+    function OPorts(nk: CNodeKind): set<CPort>
+    {
+        match nk
+        case CHier(subc) =>
+            set n | n < subc.NodeBound && subc.NodeKind(n) == Some(COutput) :: n as CPort
+        case CComb(iports, oports, path_exists, behav, names) => Seq.ToSet(oports)
+        case CInput() => {0 as CPort}
+        case COutput() => {}
+        case CConst(v) => {0 as CPort}
+        case CSeq() => {0 as CPort}
+    }
+
+    predicate IsOPort(nk: CNodeKind, p: CPort)
+    {
+        match nk
+        // The port numbers of a hierarical block and just the node ids of
+        // the input and output nodes.
+        case CHier(subc) =>
+            subc.NodeKind(p as CNode) == Some(COutput)
+        case CComb(iports, oports, path_exists, behav, names) => p in oports
+        case CInput() => p == OUTPUT_PORT as CPort
+        case CConst(v) => p == OUTPUT_PORT as CPort
+        case COutput() => false
+        case CSeq() => p == OUTPUT_PORT as CPort
+    }
+
+    ghost predicate CNodeKindSomewhatValid(nk: CNodeKind)
+    {
+        (
+        match nk
+        case CComb(iports, oports, path_exists, behav, names) =>
+          (forall a: CPort, b: CPort ::
+              (a !in oports ==> !nk.PathExists(a, b)) &&
+              (b !in iports ==> !nk.PathExists(a, b)))
+        case _ => true
+        ) && (
+            forall p: CPort ::
+                !(IsIPort(nk, p) && IsOPort(nk, p))
+        )
+    }
+
+    ghost predicate CNodeKindValid(
+        hier_level: nat, port_bound: CPort, nk: CNodeKind)
+        decreases hier_level, 0
+    {
+        CNodeKindSomewhatValid(nk) &&
+        (
+        match nk
+        case CHier(subc) =>
+            (subc.HierLevel < hier_level) &&
+            CircuitValid(subc)
+        case _ => true
+        ) && (
+            forall p: CPort ::
+                (IsIPort(nk, p) ==> p < port_bound) &&
+                (IsOPort(nk, p) ==> p < port_bound)
+        )
+    }
+
+    ghost predicate {:opaque} CircuitValid(c: Circuit)
+        decreases  c.HierLevel, 2
+    {
+        CircuitNodeKindValid(c) &&
+        CircuitPortSourceValid(c)
+    }
+
+    ghost predicate CircuitNodeKindValid(c: Circuit)
+        decreases  c.HierLevel, 1
+    {
+        (
+            forall n: CNode ::
+                var maybe_nk := c.NodeKind(n);
+                if maybe_nk.None? then
+                    true
+                else
+                    CNodeKindValid(c.HierLevel, c.PortBound, maybe_nk.Extract())
+        ) && (
+            forall n: CNode :: n >= c.NodeBound ==> c.NodeKind(n) == None
+        )
+    }
+
+    ghost predicate CircuitPortSourceValid(c: Circuit)
+    {
+        // For all possible ports.
+        // If the port is not a valid output port then PortSource should give None.0
+        // If the port is a valid output port then it should lead to a valid input
+        // port.
+        forall n: CNode ::
+            forall p: CPort ::
+                var inp := NP(n, p);
+                if NPValidInput(c, inp) then
+                    match c.PortSource(inp)
+                    // It's ok if it doesn't connect to anything.
+                    // We consider that a valid circuit, but not a complete circuit.
+                    // That way we can build a circuit but it is still valid.
+                    case None => true
+                    case Some(onp) => NPValidOutput(c, onp)
+                else
+                    c.PortSource(inp) == None
+    }
+
+    ghost predicate NPValid(c: Circuit, np: NP)
+    {
+        NPValidInput(c, np) || NPValidOutput(c, np)
+    }
+
+    ghost predicate NPValidInput(c: Circuit, np: NP)
+    {
+        match c.NodeKind(np.n)
+        // The node doesn't exist.
+        case None => false
+        case Some(nk) => IsIPort(nk, np.p)
+    }
+
+    ghost predicate NPValidOutput(c: Circuit, np: NP)
+    {
+        match c.NodeKind(np.n)
+        case None => false
+        case Some(nk) => IsOPort(nk, np.p)
+    }
+}
