Circuit/CircuitDeprecated.dfy
@@ -1,0 +1,187 @@
+module CircuitUtils {
+
+
+    import opened CircuitBase
+    import opened CircuitValidity
+    import opened CircuitHierarchy
+    import SeqNatToNat
+    import opened Std.Wrappers
+    import Std.Collections.Seq
+    import SeqExt
+
+    const MAX_HIERLEVEL := 128
+
+
+    function CircuitIPorts(c: Circuit) : set<CNode>
+    {
+        set n | n < c.NodeBound && c.NodeKind(n) == Some(CInput)
+    }
+
+    function CircuitOPorts(c: Circuit) : set<CNode>
+    {
+        set n | n < c.NodeBound && c.NodeKind(n) == Some(COutput)
+    }
+
+
+    function HierarchyPathSubcircuit(c: Circuit, hp: HierarchyPath): (r: Option<Circuit>)
+        requires CircuitValid(c)
+        requires HierarchyPathValid(c, hp)
+        decreases |hp.v|, 1
+    {
+        if HPLength(hp) == 0 then
+            None
+        else
+            var tail := HPTail(hp);
+            var n := HPHead(hp);
+            assert HierarchyPathValid(c, tail);
+            var tail_c := HierarchyPathCircuit(c, tail);
+            HierarchyPathCircuitValid(c, tail);
+            assert CircuitValid(tail_c);
+            reveal CircuitValid();
+            var nk := tail_c.NodeKind(n).value;
+            assert CircuitNodeKindValid(tail_c);
+            assert CNodeKindValid(tail_c.HierLevel, tail_c.PortBound, nk);
+            Some(tail_c.NodeKind(n).value.c)
+    }
+
+
+    ghost predicate HPNodeValid(c: Circuit, hpn: HPNode)
+        requires CircuitValid(c)
+    {
+        HierarchyPathValid(c, hpn.hp) &&
+        var hp_c := HierarchyPathCircuit(c, hpn.hp);
+        var maybe_nk := hp_c.NodeKind(hpn.n);
+        HierarchyPathValid(c, hpn.hp) && maybe_nk.Some?
+    }
+
+    ghost predicate HPNodeIsLeaf(c: Circuit, hpn: HPNode)
+        requires CircuitValid(c)
+        requires HPNodeValid(c, hpn)
+    {
+        var hp_c := HierarchyPathCircuit(c, hpn.hp);
+        var maybe_nk := hp_c.NodeKind(hpn.n);
+        !maybe_nk.value.CHier?
+    }
+
+    function CompleteHierarchyPath(c: Circuit, hp: HierarchyPath, n: CNode): (r: HPNode)
+        requires CircuitValid(c)
+        requires HierarchyPathValid(c, hp)
+        requires HierarchyPathCircuit(c, hp).NodeKind(n).Some?
+        requires !HierarchyPathCircuit(c, hp).NodeKind(n).value.CHier?
+        ensures HPNodeValid(c, r)
+    {
+        HPNode(hp, n)
+    }
+
+
+    ghost predicate CircuitPortSourceComplete(c: Circuit)
+        requires CircuitPortSourceValid(c)
+    {
+        forall n: CNode ::
+            forall p: CPort ::
+                var inp := NP(n, p);
+                if NPValidInput(c, inp) then
+                    match c.PortSource(inp)
+                    case None => false
+                    case Some(onp) => NPValidOutput(c, onp)
+                else
+                    assert c.PortSource(inp) == None;
+                    true
+    }
+    lemma HierLevelDecreases(c: Circuit, n: CNode)
+        requires c.NodeKind(n).Some?
+        requires c.NodeKind(n).value.CHier?
+        requires
+            CircuitValid(c)
+        ensures NodeToSubcircuit(c, n).HierLevel < c.HierLevel
+    {
+        reveal CircuitValid();
+        assert CircuitNodeKindValid(c);
+    }
+
+    lemma SubCircuitValid(c: Circuit, n: CNode)
+        requires
+            var maybe_nk := c.NodeKind(n);
+            (maybe_nk.Some?) &&
+            var nk := maybe_nk.Extract();
+            (nk.CHier?)
+        requires
+            CircuitValid(c)
+        ensures CircuitValid(NodeToSubcircuit(c, n))
+    {
+        reveal CircuitValid();
+        assert CircuitNodeKindValid(c);
+    }
+
+    function HPNodeToNK(c: Circuit, hpn: HPNode): CNodeKind
+        requires CircuitValid(c)
+        requires HPNodeValid(c, hpn)
+    {
+        HierarchyPathCircuit(c, hpn.hp).NodeKind(hpn.n).value
+    }
+
+    function MaxSubcircuitNodeBoundInternal(c: Circuit, n: CNode, max: nat): nat
+        requires CircuitValid(c)
+        decreases c.HierLevel, 0, n
+    {
+        var new_max := if n == 0 then max else MaxSubcircuitNodeBoundInternal(c, n-1, max);
+        match c.NodeKind(n)
+            case Some(CHier(_)) =>
+                HierLevelDecreases(c, n);
+                SubCircuitValid(c, n);
+                var next_c := NodeToSubcircuit(c, n);
+                var nb := CircuitMaxNodeBound(next_c) as nat;
+                if nb > new_max then max else nb
+            case _ => new_max
+    }
+
+    function MaxSubcircuitNodeBound(c: Circuit): nat
+        requires CircuitValid(c)
+        decreases c.HierLevel, 1
+    {
+        MaxSubcircuitNodeBoundInternal(c, c.NodeBound, 0)
+    }
+
+    function CircuitMaxNodeBound(c: Circuit): nat
+        requires CircuitValid(c)
+        decreases c.HierLevel, 2
+    {
+        // The local NodeBound get expanded.
+        var subcircuit_nb := MaxSubcircuitNodeBound(c);
+        // Just combine the max node bound on this level with the max node bound on the next level
+        SeqNatToNat.NatsToNat([c.NodeBound as nat, subcircuit_nb as nat])
+    }
+
+    //function Subcircuits(c: Circuit): seq<Circuit>
+    //{
+    //    seq(n requires 0 <= n < c.NodeBound | c.NodeKind(n).Some? && c.NodeKind(n).value.CHier? :: c.NodeKind(n).value.Circuit)
+    //}
+
+    //function MaxSubcircuitMaxPortBoundInternal(c: Circuit, n: CNode, max: nat): nat
+    //    requires CircuitValid(c)
+    //    decreases c.HierLevel, 0, n
+    //{
+    //    var new_max := if n == 0 then max else MaxSubcircuitMaxPortBoundInternal(c, n-1, max);
+    //    match c.NodeKind(n)
+    //        case Some(CHier(_)) =>
+    //            HierLevelDecreases(c, n);
+    //            SubCircuitValid(c, n);
+    //            var next_c := NodeToSubcircuit(c, n);
+    //            var nb := CircuitMaxPortBound(next_c);
+    //            if nb > new_max then max else nb
+    //        case _ => new_max
+    //}
+
+    //function MaxSubcircuitMaxPortBound(c: Circuit): nat
+    //    requires CircuitValid(c)
+    //    decreases c.HierLevel, 1
+    //{
+    //    MaxSubcircuitMaxPortBoundInternal(c, c.NodeBound, 0)
+    //}
+
+    // Show that if there is a path in the Circuit there is a path in the HGraph.
+    // Show that if there is not a path in the Circuit there is no path in the HGraph.
+
+
+
+}
