Circuit/CircuitHierarchy.dfy
@@ -1,0 +1,218 @@
+module CircuitHierarchy {
+
+    import opened CircuitBase
+    import opened CircuitValidity
+
+    predicate HierarchyPathValid(c: Circuit, hp: HierarchyPath)
+        requires CircuitValid(c)
+        decreases |hp.v|, 0
+    {
+        if HPLength(hp) == 0 then
+            true
+        else
+            var (head, tail) := HPHeadTail(hp);
+            HierarchyPathValid(c, tail) &&
+            var hp_c := HierarchyPathCircuit(c, tail);
+            hp_c.NodeKind(head).Some? && hp_c.NodeKind(head).value.CHier?
+    }
+
+    function HPLength(hp: HierarchyPath): nat
+    {
+        |hp.v|
+    }
+
+    function HierarchyPathCircuit(c: Circuit, hp: HierarchyPath): (r: Circuit)
+        requires CircuitValid(c)
+        requires HierarchyPathValid(c, hp)
+        decreases |hp.v|, 1
+    {
+        if HPLength(hp) == 0 then
+            c
+        else
+            var tail := HPTail(hp);
+            var n := HPHead(hp);
+            assert HierarchyPathValid(c, tail);
+            var tail_c := HierarchyPathCircuit(c, tail);
+            HierarchyPathCircuitValid(c, tail);
+            //var cref := tail_c.NodeKind(n).value.CRef;
+            //tail_c.Subcircuits[cref]
+            assert CircuitValid(tail_c);
+            var nk := tail_c.NodeKind(n).value;
+            reveal CircuitValid();
+            assert CircuitNodeKindValid(tail_c);
+            assert CNodeKindValid(tail_c.HierLevel, tail_c.PortBound, nk);
+            NodeToSubcircuit(tail_c, n)
+    }
+
+
+    function HPTail(hp: HierarchyPath): (r: HierarchyPath)
+        requires hp.v != []
+        ensures |hp.v| == |r.v| + 1
+    {
+        HP(hp.v[..|hp.v|-1])
+    }
+
+    function HPHead(hp: HierarchyPath): CNode
+        requires hp.v != []
+    {
+        hp.v[|hp.v|-1]
+    }
+
+    function HPHeadTail(hp: HierarchyPath): (r: (CNode, HierarchyPath))
+        requires HPLength(hp) > 0
+    {
+        (HPHead(hp), HPTail(hp))
+    }
+
+    function HPStartChildren(hp: HierarchyPath): (r: (CNode, HierarchyPath))
+        requires HPLength(hp) > 0
+    {
+        (hp.v[0], HP(hp.v[1..]))
+    }
+
+    lemma HierarchyPathCircuitValid(c: Circuit, hp: HierarchyPath)
+        requires CircuitValid(c)
+        requires HierarchyPathValid(c, hp)
+        ensures CircuitValid(HierarchyPathCircuit(c, hp))
+        decreases |hp.v|
+    {
+        if HPLength(hp) == 0 {
+            assert HierarchyPathCircuit(c, hp) == c;
+        } else {
+            var tail := HPTail(hp);
+            assert HierarchyPathValid(c, tail);
+            var tail_c := HierarchyPathCircuit(c, tail);
+            HierarchyPathCircuitValid(c, tail);
+            assert CircuitValid(tail_c);
+            reveal CircuitValid();
+            assert CircuitNodeKindValid(tail_c);
+            var hp_c := HierarchyPathCircuit(c, hp);
+            assert CircuitValid(hp_c);
+        }
+    }
+
+    function NodeToSubcircuit(c: Circuit, n: CNode): Circuit
+        requires c.NodeKind(n).Some?
+        requires c.NodeKind(n).value.CHier?
+    {
+        c.NodeKind(n).value.c
+    }
+
+    predicate {:opaque} HPNPValidInput(c: Circuit, hpnp: HPNP)
+        requires CircuitValid(c)
+    {
+        HierarchyPathValid(c, hpnp.hpn.hp) &&
+        var hp_c := HierarchyPathCircuit(c, hpnp.hpn.hp);
+        var maybe_nk := hp_c.NodeKind(hpnp.hpn.n);
+        maybe_nk.Some? &&
+        IsIPort(maybe_nk.value, hpnp.p)
+    }
+
+    lemma HPNPValidHPValid(c: Circuit, hpnp: HPNP)
+        requires CircuitValid(c)
+        requires HPNPValid(c, hpnp)
+        ensures HierarchyPathValid(c, hpnp.hpn.hp)
+    {
+        reveal HPNPValidInput();
+        reveal HPNPValidOutput();
+    }
+
+
+    predicate {:opaque} HPNPValidOutput(c: Circuit, hpnp: HPNP)
+        requires CircuitValid(c)
+    {
+        HierarchyPathValid(c, hpnp.hpn.hp) &&
+        var hp_c := HierarchyPathCircuit(c, hpnp.hpn.hp);
+        var maybe_nk := hp_c.NodeKind(hpnp.hpn.n);
+        maybe_nk.Some? &&
+        IsOPort(maybe_nk.value, hpnp.p)
+    }
+
+    lemma HPNPNotBothValidInputOutput(c: Circuit, hpnp: HPNP)
+        requires CircuitValid(c)
+        requires HPNPValid(c, hpnp)
+        ensures !(HPNPValidOutput(c, hpnp) && HPNPValidInput(c, hpnp))
+    {
+        reveal HPNPValidInput();
+        reveal HPNPValidOutput();
+        assert HierarchyPathValid(c, hpnp.hpn.hp);
+        var hp_c := HierarchyPathCircuit(c, hpnp.hpn.hp);
+        HierarchyPathCircuitValid(c, hpnp.hpn.hp);
+        var nk := hp_c.NodeKind(hpnp.hpn.n).value;
+        reveal CircuitValid();
+        assert CircuitNodeKindValid(hp_c);
+    }
+
+    predicate HPNPValid(c: Circuit, hpnp: HPNP)
+        requires CircuitValid(c)
+    {
+        HPNPValidInput(c, hpnp) ||
+        HPNPValidOutput(c, hpnp)
+    }
+
+
+    function HPNPtoNK(c: Circuit, hpnp: HPNP): (r: CNodeKind)
+        requires CircuitValid(c)
+        requires HPNPValid(c, hpnp)
+        ensures
+            reveal HPNPValidInput();
+            reveal HPNPValidOutput();
+            var hp_c := HierarchyPathCircuit(c, hpnp.hpn.hp);
+            var nk := HPNPtoNK(c, hpnp);
+            CNodeKindValid(hp_c.HierLevel, hp_c.PortBound, nk)
+    {
+        HPNPValidHPValid(c, hpnp);
+        var hp_c := HierarchyPathCircuit(c, hpnp.hpn.hp);
+        HierarchyPathCircuitValid(c, hpnp.hpn.hp);
+        reveal HPNPValidInput();
+        reveal HPNPValidOutput();
+        var nk := hp_c.NodeKind(hpnp.hpn.n).value;
+        CircuitValidCNodeKindValid(hp_c, hpnp.hpn.n);
+        nk
+    }
+
+    lemma CircuitValidCNodeKindValid(c: Circuit, n: CNode)
+        requires CircuitValid(c)
+        requires c.NodeKind(n).Some?
+        ensures CNodeKindValid(c.HierLevel, c.PortBound, c.NodeKind(n).value)
+    {
+        reveal CircuitValid();
+    }
+    ghost predicate {:opaque} CircuitComplete(c: Circuit)
+        requires CircuitValid(c)
+        decreases c.HierLevel
+    {
+        (forall inp: NP :: NPValidInput(c, inp) ==> c.PortSource(inp).Some?) &&
+        (forall n: CNode :: c.NodeKind(n).Some? && c.NodeKind(n).value.CHier? ==>
+            var subc := c.NodeKind(n).value.c;
+            CircuitValid(subc) &&
+            (subc.HierLevel < c.HierLevel) &&
+            CircuitComplete(subc)
+        )
+    }
+
+    predicate CNodeIsCHier(c: Circuit, n: CNode)
+        requires CircuitValid(c)
+    {
+        c.NodeKind(n).Some? && c.NodeKind(n).value.CHier?
+    }
+
+    function DirectSubcircuits(c: Circuit): (r: seq<Circuit>)
+        requires CircuitValid(c)
+    {
+        reveal CircuitValid();
+        assert CircuitNodeKindValid(c);
+        assert forall i: CNode ::
+            i < c.NodeBound && c.NodeKind(i).Some? && c.NodeKind(i).value.CHier? ==>
+            var nk := c.NodeKind(i).value;
+            CNodeKindValid(c.HierLevel, c.PortBound, nk);
+        var all_cnodes := seq(c.NodeBound, (i: nat) requires i < c.NodeBound as nat => i as CNode);
+        var all_subcircuit_cnodes := Seq.Filter(n => CNodeIsCHier(c, n), all_cnodes);
+        var all_subcircuits := Seq.Map(
+            i requires CNodeIsCHier(c, i) => c.NodeKind(i).value.c, all_subcircuit_cnodes);
+        all_subcircuits
+    }
+
+
+
+}
