Circuit/CircuitPortBounds.dfy
@@ -1,0 +1,169 @@
+module CircuitPortBounds
+{
+
+    import opened Std.Wrappers
+    import opened Std.Collections.Seq
+    import opened CircuitBase
+    import opened CircuitHierarchy
+
+    function PortListBound(pl: seq<CPort>): CPort
+    {
+        if |pl| == 0 then
+            0 as CPort
+        else
+            var pl_nat := seq(|pl|, (index: nat) requires index < |pl| => pl[index] as nat);
+            var m: nat := Seq.Max(pl_nat);
+            m as CPort
+    }
+
+    lemma NKPortBoundBinds(nk: CNodeKind)
+        ensures 
+            var bound := NKPortBound(nk);
+            forall p: CPort ::
+                (IsIPort(nk, p) ==> p < bound) &&
+                (IsOPort(nk, p) ==> p < bound)
+    {
+        var bound := NKPortBound(nk);
+        match nk
+        case CHier(subc) => {
+            assert forall p: CPort ::
+                (IsIPort(nk, p) ==> p < bound) &&
+                (IsOPort(nk, p) ==> p < bound);
+        }
+        case CComb(iports, oports, path_exists, behav, name) => {
+            assert forall p: CPort ::
+                (IsIPort(nk, p) ==> p < bound) &&
+                (IsOPort(nk, p) ==> p < bound);
+        }
+        case CInput() => {
+        }
+        case CConst(v) =>  {
+        }
+        case COutput() => {
+        } 
+        case CSeq() => {
+            assert forall p: CPort ::
+                (IsIPort(nk, p) ==> p < bound) &&
+                (IsOPort(nk, p) ==> p < bound);
+        }
+    }
+
+    function MaxNodeInternal(c: Circuit, f: CNode -> bool, n: CNode): (r: Option<CNode>)
+        ensures r.None? ==> !exists m: CNode :: m <= n && f(m)
+        ensures r.Some? ==> !exists m: CNode :: m > r.value && m <= n && f(m)
+        decreases n
+    {
+        if f(n) then
+            Some(n)
+        else
+            if n == 0 then
+                None
+            else
+                MaxNodeInternal(c, f, n-1)
+    }
+
+    function CInputNodeBound(c: Circuit): (r: CNode)
+        requires CircuitValid(c)
+        ensures forall n: CNode ::
+            c.NodeKind(n).Some? && c.NodeKind(n).value.CInput? ==>
+            n < r
+    {
+        reveal CircuitValid();
+        assert forall n: CNode ::
+            c.NodeKind(n).Some? ==> n < c.NodeBound;
+        var maybe_n := MaxNodeInternal(c, n => c.NodeKind(n).Some? && c.NodeKind(n).value.CInput?, c.NodeBound-1);
+        match maybe_n
+        case None => 0
+        case Some(n) => n + 1
+    }
+
+    function COutputNodeBound(c: Circuit): (r: CNode)
+        ensures forall n: CNode ::
+            c.NodeKind(n).Some? && c.NodeKind(n).value.COutput? ==>
+            n < r
+    {
+        var maybe_n := MaxNodeInternal(c, n => c.NodeKind(n).Some? && c.NodeKind(n).value.COutput?, c.NodeBound-1);
+        match maybe_n
+        case None => 0
+        case Some(n) => n + 1
+    }
+
+
+    function NKPortBound(nk: CNodeKind): CPort
+    {
+        var bound := match nk
+        case CHier(c) =>
+            var max_i := CInputNodeBound(c);
+            var max_o := COutputNodeBound(c);
+            (if max_i > max_o then max_i else max_o) as CPort
+        case CComb(iports, oports, _, _, _) =>
+            var max_i := PortListBound(iports);
+            var max_o := PortListBound(oports);
+            if max_i > max_o then max_i+1 else max_o+1
+        case CConst(_) => OUTPUT_PORT +1
+        case CInput() => OUTPUT_PORT +1
+        case COutput() => INPUT_PORT +1
+        case CSeq() => (if INPUT_PORT > OUTPUT_PORT then INPUT_PORT else OUTPUT_PORT)+1;
+        bound
+    }
+
+    ghost function CircuitMaxPortBound(c: Circuit): nat
+        requires CircuitValid(c)
+        decreases c.HierLevel, 2
+    {
+        var subcircuits: seq<Circuit> := HierSubcircuits(c);
+        var port_bounds := (set c: Circuit | c in subcircuits :: c.PortBound as nat);
+        if |port_bounds| == 0 then
+            c.PortBound as nat
+        else
+            var max_hier_port_bound := MaxInSet(port_bounds);
+            if c.PortBound as nat > max_hier_port_bound then c.PortBound as nat else max_hier_port_bound
+    }
+
+    ghost function HierSubcircuitsInternal(
+        hier_level: nat, new_cs: seq<Circuit>, old_cs: seq<Circuit>): (r: seq<Circuit>)
+        requires forall x :: x in new_cs ==> x.HierLevel < hier_level
+        requires forall x :: x in new_cs ==> CircuitValid(x)
+        decreases hier_level, 0, |new_cs|
+     {
+        if |new_cs| == 0 then
+            old_cs
+        else
+            var head: Circuit := new_cs[0];
+            var tail: seq<Circuit> := new_cs[1..];
+            var expanded := HierSubcircuits(head);
+            HierSubcircuitsInternal(hier_level, tail, old_cs + expanded)
+     }
+ 
+     ghost function HierSubcircuits(c: Circuit): (r: seq<Circuit>)
+         requires CircuitValid(c)
+         decreases c.HierLevel, 1
+     {
+         var direct := DirectSubcircuits(c);
+         reveal CircuitValid();
+         assert CircuitNodeKindValid(c);
+         HierSubcircuitsInternal(c.HierLevel, direct, direct)
+     }
+
+    ghost function MaxInSetInternal(a: set<nat>, max: nat): nat
+    {
+        if |a| == 0 then
+            max
+        else
+            var y :| y in a;
+            MaxInSetInternal(
+                a - {y},
+                if y > max then y else max
+            )
+    }
+
+    ghost function MaxInSet(a: set<nat>): nat
+        requires |a| > 0
+    {
+        var y :| y in a;
+        MaxInSetInternal(a - {y}, y)
+    }
+
+
+
+}
