Circuit/CircuitToGraph.dfy
@@ -1,0 +1,165 @@
+module CircuitToGraph {
+
+    import DG = DigraphBase
+    import DP = DigraphPaths
+    import opened Std.Wrappers
+    import opened CircuitBase
+    import opened CircuitHierarchy
+    import opened CircuitHPNP
+    import opened CircuitNodeBounds
+
+    // INP and ONP reference ports on a single level of the hierarchy.
+    // The 'n' can point at an internal node, or at a port on the external
+    // interface.
+
+
+    function {:opaque} CtoG(c: Circuit): (g: DG.Digraph<HPNP>)
+        requires CircuitValid(c)
+    {
+        DG.Digraph(
+            hpnp => HPNPValid(c, hpnp),
+            (a, b) => HPNPConnected(c, a, b),
+            HPNPToNat,
+            NatToHPNP,
+            HPNPBound(c)
+        )
+    }
+
+    function CtoGV(c: Circuit): (g: DG.Digraph<HPNP>)
+        requires CircuitValid(c)
+        ensures DG.DigraphValid(g)
+    {
+        CtoGValid(c);
+        CtoG(c)
+    }
+
+    function {:vcs_split_on_every_assert} HPINPtoHPONP(c: Circuit, hpinp: HPNP) : (r: Option<HPNP>)
+        requires CircuitValid(c)
+        requires HPNPValidInput(c, hpinp)
+        ensures r.None? || HPNPValid(c, r.value)
+    {
+        var hp := hpinp.hpn.hp;
+        HPNPValidHPValid(c, hpinp);
+        var parent_c := HierarchyPathCircuit(c, hp);
+        HierarchyPathCircuitValid(c, hp);
+        assert CircuitValid(parent_c);
+        reveal HPNPValidOutput();
+        reveal CircuitValid();
+        assert CircuitNodeKindValid(parent_c);
+        assert CircuitPortSourceValid(parent_c);
+        var inp := NP(hpinp.hpn.n, hpinp.p);
+        reveal HPNPValidInput();
+        assert NPValidInput(parent_c, inp);
+        var maybe_onp: Option<NP> := parent_c.PortSource(inp);
+            match maybe_onp
+            // The input port does not connect to anything.
+            case None => None
+            // The input port does connect.
+            case Some(onp) =>
+                assert NPValid(parent_c, onp);
+                assert NPValidOutput(parent_c, onp);
+                var nk := parent_c.NodeKind(onp.n);
+                assert nk.Some?;
+                assert IsOPort(nk.value, onp.p);
+                var hpn := HPNode(hp, onp.n);
+                var hpnp := HPNP(hpn, onp.p);
+                reveal HPNPValidOutput();
+                assert HPNPValidOutput(c, hpnp);
+                Some(hpnp)
+    }
+
+    function NumberOfRemainingNodes(c: Circuit, seen_path: DG.Path<HPNP>): nat
+        requires CircuitValid(c)
+        requires CircuitNoLoops(c)
+        requires PathValid(c, seen_path)
+    {
+        DP.NoLoopsMeansNoRepeats(CtoGV(c));
+        DP.NumberOfRemainingNodesPath(CtoGV(c), seen_path)
+    }
+
+    lemma NumberOfRemainingNodesDecreases(c: Circuit, seen_path: DG.Path<HPNP>, n: HPNP)
+        requires CircuitValid(c)
+        requires CircuitNoLoops(c)
+        requires PathValid(c, seen_path)
+        requires HPNPValid(c, n)
+        requires |seen_path.v| > 0 ==> HPNPConnected(c, DP.PathEnd(seen_path), n)
+        ensures
+            var new_p := PathAppend(c, seen_path, n);
+            NumberOfRemainingNodes(c, new_p) <
+            NumberOfRemainingNodes(c, seen_path)
+    {
+        DP.NoLoopsMeansNoRepeats(CtoGV(c));
+        assert DP.PathNoRepeats(seen_path);
+    }
+
+    lemma CtoGValid(c: Circuit)
+        requires CircuitValid(c)
+        ensures DG.DigraphValid(CtoG(c))
+    {
+        reveal CtoG();
+        var g := CtoG(c);
+        forall n: HPNP, m: HPNP
+            ensures HPNPToNat(n) >= HPNPBound(c) ==> !HPNPValid(c, n)
+            ensures !HPNPConnected(c, n, n)
+            ensures HPNPConnected(c, n, m) ==> HPNPValid(c, n) && HPNPValid(c, m)
+            ensures (n != m) ==> HPNPToNat(n) != HPNPToNat(m)
+        {
+            OutOfBoundInvalid(c, n);
+            NoSelfConnections(c, n);
+            ConnectedNodesValid(c, n, m);
+            HPNPToNatInjective(n, m);
+        }
+        assert (forall n: HPNP :: HPNPToNat(n) >= HPNPBound(c) ==> !HPNPValid(c, n));
+        assert (forall n: HPNP :: !HPNPConnected(c, n, n));
+        assert (forall n: HPNP, m: HPNP :: HPNPConnected(c, n, m) ==> HPNPValid(c, n) && HPNPValid(c, m));
+        assert (forall n: HPNP, m: HPNP :: n != m ==> HPNPToNat(n) != HPNPToNat(m));
+        reveal DG.DigraphValid();
+    }
+    
+    ghost predicate CircuitNoLoops(c: Circuit)
+        requires CircuitValid(c)
+    {
+        var g := CtoG(c);
+        !DG.DigraphLoop(g)
+    }
+
+    lemma NoLoopsMeansNotInPath(c: Circuit, p: DG.Path<HPNP>, n: HPNP)
+        requires CircuitValid(c)
+        requires CircuitNoLoops(c)
+        requires PathValid(c, p)
+        requires HPNPValid(c, n)
+        requires |p.v| > 0 ==> HPNPConnected(c, DP.PathEnd(p), n)
+        ensures n !in p.v
+    {
+        var new_p := PathAppend(c, p, n);
+        assert new_p == DG.Path(p.v + [n]);
+        assert PathValid(c, new_p);
+        DG.NoLoopsMeansNoRepeats(CtoGV(c));
+        assert DG.PathNoRepeats(new_p);
+        if n in p.v {
+            var index: nat :| index < |p.v| && p.v[index] == n;
+            assert new_p.v[index] == n;
+            assert new_p.v[|new_p.v|-1] == n;
+            assert !DG.PathNoRepeats(new_p);
+        }
+    }
+
+    function PathAppend(c: Circuit, p: DG.Path<HPNP>, n: HPNP): (r: DG.Path<HPNP>)
+        // Just a PathAppend with more friendly requirements for a circuit.
+        requires CircuitValid(c)
+        requires DG.PathValid(CtoGV(c), p)
+        requires HPNPValid(c, n)
+        requires (|p.v| > 0 ==> HPNPConnected(c, DG.PathEnd(p), n))
+        ensures DG.PathValid(CtoGV(c), r)
+    {
+        reveal CtoG();
+        DG.PathAppend(CtoGV(c), p, n)
+    }
+
+    predicate PathValid(c: Circuit, seen_path: DG.Path<HPNP>)
+        requires CircuitValid(c)
+    {
+        DG.PathValid(CtoGV(c), seen_path)
+    }
+    
+}
