Digraph/DigraphAddNode.dfy
@@ -1,0 +1,116 @@
+module DigraphAddNode {
+
+    import opened DigraphBase
+    import opened DigraphPaths
+    // Adding nodes
+
+    function AddNode<Node(==)>(g: Digraph, n: Node): (r: Digraph)
+        requires !g.IsNode(n)
+    {
+        Digraph(
+            m=>(m==n) || g.IsNode(m),
+            g.IsConnected,
+            g.NodeMap,
+            g.InvNodeMap,
+            if g.NodeMap(n) >= g.NodeBound then g.NodeMap(n)+1 else g.NodeBound
+        )
+    }
+
+    lemma AddNodeDigraphValid<Node>(g: Digraph, n: Node)
+        requires DigraphValid(g)
+        requires !g.IsNode(n)
+        ensures
+            var r := AddNode(g, n);
+            DigraphValid(r)
+    {
+        reveal DigraphValid();
+    }
+
+    function AddNodeV<Node(==)>(g: Digraph, n: Node): (r: Digraph)
+        requires DigraphValid(g)
+        requires !g.IsNode(n)
+        ensures
+            DigraphValid(r)
+    {
+        AddNodeDigraphValid(g, n);
+        AddNode(g, n)
+    }
+
+    lemma AddNodePathValidHelper<Node>(r: Digraph, n: Node, x: Node)
+        requires (forall m: Node :: !r.IsConnected(n, m))
+        requires (forall m: Node :: !r.IsConnected(m, n))
+        ensures !r.IsConnected(n, x)
+        ensures !r.IsConnected(x, n)
+    {
+    }
+    
+    // There is only one path that becomes valid when we add a node.
+    // It is the path containing just that node.
+    lemma AddNodePathValid<Node>(g: Digraph, n: Node, p: Path<Node>)
+        requires DigraphValid(g)
+        requires !g.IsNode(n)
+        ensures
+            var r := AddNode(g, n);
+            (PathValid(g, p) ==> PathValid(r, p)) &&
+            (PathValid(r, p) ==> PathValid(g, p) || p == Path([n])) &&
+            true
+    {
+        var r := AddNode(g, n);
+        reveal PathValid();
+        reveal DigraphValid();
+        assert forall m: Node :: !g.IsConnected(m, n);
+        assert forall m: Node :: !g.IsConnected(n, m);
+        assert forall m: Node :: !r.IsConnected(m, n);
+        assert forall m: Node :: !r.IsConnected(n, m);
+        if n in p.v {
+            assert !PathValid(g, p);
+            if |p.v| == 1 {
+                assert PathValid(r, p);
+            } else {
+                if p.v[0] == n {
+                    AddNodePathValidHelper(r, n, p.v[1]);
+                    assert !r.IsConnected(p.v[0], p.v[1]);
+                    assert !PathValid(r, p);
+                } else {
+                    var index := PathFindIndex(p, n);
+                    AddNodePathValidHelper(r, n, p.v[index-1]);
+                    assert !r.IsConnected(p.v[index-1], p.v[index]);
+                    assert !PathValid(r, p);
+                }
+                assert !PathValid(r, p);
+            }
+        } else {
+        }
+    }
+
+    /*
+    When we add a node to a graph, that cannot introduce any loops.
+    */
+    lemma AddNodeLoopConserved<Node(!new)>(g: Digraph, n: Node)
+        requires DigraphValid(g)
+        requires !g.IsNode(n)
+        ensures
+            var r := AddNode(g, n);
+            DigraphLoop(g) == DigraphLoop(r)
+    {
+        var r := AddNode(g, n);
+        reveal PathValid();
+        reveal DigraphLoop();
+        if DigraphLoop(g) {
+            var p := GetLoopPath(g);
+            assert PathValid(r, p);
+            assert DigraphLoop(r);
+        }
+        if DigraphLoop(r) {
+            var p :| PathValid(r, p) && PathLoop(p);
+            AddNodePathValid(g, n, p);
+            assert PathValid(g, p) || p == Path([n]);
+            if p == Path([n]) {
+                assert !PathLoop(p);
+            }
+            assert PathValid(g, p);
+            assert DigraphLoop(g);
+        }
+    }
+    
+}
