Digraph/DigraphBase.dfy
@@ -1,0 +1,76 @@
+module DigraphBase {
+
+    import opened Std.Wrappers
+    import Std.Functions
+    import Std.Collections.Set
+
+    datatype Path<Node> = Path(v: seq<Node>)
+
+    datatype Digraph<!Node> = Digraph(
+        IsNode: Node -> bool,
+        IsConnected: (Node, Node) -> bool,
+        NodeMap: Node -> nat,
+        InvNodeMap: nat -> Option<Node>,
+        NodeBound: nat
+    )
+
+    ghost predicate {:opaque} DigraphValid<Node(!new)>(g: Digraph)
+    {
+        (forall n: Node :: g.NodeMap(n) >= g.NodeBound ==> !g.IsNode(n)) &&
+        (forall n: Node :: !g.IsConnected(n, n)) && // No self-connections
+        (forall n: Node, m: Node :: g.IsConnected(n, m) ==> g.IsNode(n) && g.IsNode(m)) &&
+        (forall n: Node, m: Node :: n != m ==> g.NodeMap(n) != g.NodeMap(m)) &&
+        (forall n: Node :: g.InvNodeMap(g.NodeMap(n)) == Some(n)) &&
+        Functions.Injective(g.NodeMap) && Functions.Injective(g.InvNodeMap)
+    }
+
+    lemma ValidNodeBound<Node>(g: Digraph, n: Node)
+        requires DigraphValid(g)
+        requires g.IsNode(n)
+        ensures g.NodeMap(n) < g.NodeBound
+    {
+        reveal DigraphValid();
+    }
+
+    predicate NodeValid<Node>(g: Digraph, n: Node)
+    {
+        g.NodeMap(n) < g.NodeBound
+    }
+    
+    lemma NotNodeNotConnected<Node>(g: Digraph, n: Node)
+        // If a node is not in the graph
+        // then it's not connected to any nodes
+        requires DigraphValid(g)
+        requires !g.IsNode(n)
+        ensures
+            (forall m: Node :: !g.IsConnected(m, n)) &&
+            (forall m: Node :: !g.IsConnected(n, m))
+    {
+        reveal DigraphValid();
+    }
+
+    predicate {:opaque} PathValid<Node>(g: Digraph, p: Path<Node>)
+    {
+        (forall i: nat :: i < |p.v| ==> g.IsNode(p.v[i])) &&
+        (forall i: nat :: i < |p.v|-1 ==> g.IsConnected(p.v[i], p.v[i+1]))
+    }
+    
+
+    function AllNodes<Node(!new)>(g: Digraph): (r: set<Node>)
+        requires DigraphValid(g)
+        ensures forall n: Node :: g.IsNode(n) ==> n in r
+        ensures forall n: Node :: n in r ==> g.IsNode(n)
+        ensures forall n: Node :: n in r ==> NodeValid(g, n)
+    {
+        reveal DigraphValid();
+        var mapped := set m: nat | m < g.NodeBound :: m;
+        var nodes := Set.Map(g.InvNodeMap, mapped);
+        var filter := (n: Option<Node>) => n.Some? && g.IsNode(n.value);
+        var filtered_nodes := Set.Filter(filter, nodes);
+        assert forall n :: n in filtered_nodes ==> filter(n);
+        var extracted_nodes := set n | n in filtered_nodes :: n.value;
+        extracted_nodes
+    }
+
+
+}
