Digraph/DigraphConnectNodes.dfy
@@ -1,0 +1,169 @@
+module DigraphConnectNodes {
+
+    import opened DigraphBase
+    import opened DigraphPaths
+
+    function ConnectNodes<Node(==)>(g: Digraph, n: Node, m: Node): (r: Digraph)
+        requires g.IsNode(n)
+        requires g.IsNode(m)
+        requires n != m
+        requires !g.IsConnected(n, m)
+    {
+        Digraph(
+            g.IsNode,
+            (a, b) => ((a==n) && (b==m)) || g.IsConnected(a, b),
+            g.NodeMap,
+            g.InvNodeMap,
+            g.NodeBound
+        )
+    }
+
+    lemma ConnectNodesDigraphValid<Node>(g: Digraph, n: Node, m: Node)
+        requires g.IsNode(n)
+        requires g.IsNode(m)
+        requires n != m
+        requires !g.IsConnected(n, m)
+        requires DigraphValid(g)
+        ensures
+            var r := ConnectNodes(g, n, m);
+            DigraphValid(r)
+    {
+        reveal DigraphValid();
+    }
+
+    function ConnectNodesV<Node(==)>(g: Digraph, n: Node, m: Node): (r: Digraph)
+        requires g.IsNode(n)
+        requires g.IsNode(m)
+        requires n != m
+        requires !g.IsConnected(n, m)
+        requires DigraphValid(g)
+        ensures DigraphValid(r)
+    {
+        ConnectNodesDigraphValid(g, n, m);
+        ConnectNodes(g, n, m)
+    }
+
+    lemma ConnectNodesPathStillValid<Node>(g: Digraph, n: Node, m: Node, p: Path<Node>)
+        requires g.IsNode(n) && g.IsNode(m) && n != m && !g.IsConnected(n, m)
+        requires PathValid(g, p)
+        ensures
+            var r := ConnectNodes(g, n, m);
+            PathValid(r, p)
+    {
+        reveal PathValid(); 
+    }
+
+    lemma ConnectNodesPathStillExists<Node(!new)>(
+            g: Digraph, n: Node, m: Node, a: Node, b: Node)
+        requires g.IsNode(n) && g.IsNode(m) && n != m && !g.IsConnected(n, m)
+        requires PathExists(g, a, b)
+        ensures
+            var r := ConnectNodes(g, n, m);
+            PathExists(r, a, b)
+    {
+        var r := ConnectNodes(g, n, m);
+        var p :| PathFromTo(g, p, a, b);
+        ConnectNodesPathStillValid(g, n, m, p);
+        PathExistsByExample(r, p, a, b);
+    }
+
+    lemma ConnectNodesPathExists<Node(!new)>(g: Digraph, n: Node, m: Node)
+        requires g.IsNode(n) && g.IsNode(m) && n != m && !g.IsConnected(n, m)
+        ensures
+            var r := ConnectNodes(g, n, m);
+            PathExists(r, n, m)
+    {
+        var p := Path([n, m]);
+        var r := ConnectNodes(g, n, m);
+        assert r.IsConnected(n, m);
+        reveal PathValid();
+        assert PathFromTo(r, p, n, m);
+        PathExistsByExample(r, p, n, m);
+        assert PathExists(r, n, m);
+    }
+
+    // If there was already a path from b to a then adding a connection from a to b will
+    // create a loop.
+    lemma ConnectNodesDigraphLoop<Node(!new)>(g: Digraph, n: Node, m: Node)
+        requires g.IsNode(n) && g.IsNode(m) && n != m && !g.IsConnected(n, m)
+        ensures
+            var r := ConnectNodes(g, n, m);
+            DigraphLoop(r) == DigraphLoop(g) || PathExists(g, m, n)
+    {
+        var r := ConnectNodes(g, n, m);
+        if DigraphLoop(g) {
+            reveal DigraphLoop();
+            var p: Path<Node> :| PathValid(g, p) && PathLoop(p);
+            ConnectNodesPathStillValid(g, n, m, p);
+            assert PathValid(r, p);
+            assert DigraphLoop(r);
+        }
+        ConnectNodesPathExists(g, n, m);
+        assert PathExists(r, n, m);
+        if PathExists(g, m, n) {
+            var p :| PathFromTo(g, p, m, n);
+            reveal PathValid();
+            assert PathFromTo(r, p, m, n);
+            ConnectNodesPathStillValid(g, n, m, p);
+            assert PathExists(r, m, n);
+            PathExistsAdd(r, n, m, n);
+            assert PathExists(r, n, n);
+            var q :| PathFromTo(r, q, n, n);
+            assert PathLoop(q);
+            reveal DigraphLoop();
+            assert DigraphLoop(r);
+        }
+        if DigraphLoop(r) {
+            reveal DigraphLoop();
+            if !DigraphLoop(g) {
+                var p :| PathValid(r, p) && PathLoop(p);
+                assert !PathValid(g, p);
+                reveal PathValid();
+                // First assume that n to m is not in the path.
+                // Then prove that this is not possible.
+                if !exists index: nat :: index < |p.v|-1 && (p.v[index] == n) && (p.v[index+1] == m) {
+                    forall index: nat | index < |p.v|-1
+                        ensures g.IsConnected(p.v[index], p.v[index+1])
+                    {
+                        assert r.IsConnected(p.v[index], p.v[index+1]);
+                        assert g.IsConnected(p.v[index], p.v[index+1]);
+                    }
+                    assert false;
+                }
+                assert exists index: nat :: index < |p.v|-1 && (p.v[index] == n) && (p.v[index+1] == m);
+                var index: nat :| index < |p.v|-1 && (p.v[index] == n) && (p.v[index+1] == m);
+                assert PathStart(p) == PathEnd(p);
+                var q_1 := PathSegment(p, index+1, |p.v|);
+                assert |q_1.v| > 0;
+                assert PathEnd(q_1) == p.v[|p.v|-1];
+                assert PathEnd(q_1) == PathEnd(p);
+                PathSegmentValid(r, p, index+1, |p.v|);
+                assert PathValid(r, q_1);
+                var q_2 := PathSegment(p, 0, index+1);
+                assert PathStart(q_2) == PathStart(p);
+                assert PathStart(q_2) == PathEnd(q_1);
+                PathSegmentValid(r, p, 0, index+1);
+                var q := AddPaths(q_1, q_2);
+                AddPathsValid(r, q_1, q_2);
+                assert PathValid(r, q);
+                AddPathsFromTo(r, q_1, q_2);
+                assert p.v[index+1] == m;
+                assert q_1.v[0] == m;
+                assert PathFromTo(r, q, m, n);
+                // We want to now show that [n, m] does not appear in q.
+                // We actually need to find another path that removes any repeats and then
+                // show that that does not include [n, m]
+                // Then we can show that that is valid in g.
+                var s := PathRemoveLoops(q);
+                RemoveLoopsFromToSame(r, q);
+                assert PathFromTo(r, s, m, n);
+                assert PathValid(r, s);
+                assert PathNoRepeats(s);
+                assert PathValid(g, s);
+                assert PathFromTo(g, s, m, n);
+            }
+            assert DigraphLoop(g) || PathExists(g, m, n);
+        }
+    }
+
+}
