Digraph/DigraphDeprecated.dfy
@@ -1,0 +1,383 @@
+module DigraphDeprecated {
+
+    import opened Std.Wrappers
+    import Utils
+    import SeqExt
+    import Std.Collections.Seq
+    import Std.Collections.Set
+    import Std.Functions
+
+    import opened DigraphBase
+    import opened DigraphPaths
+
+    predicate {:opaque} PathExcludes<Node>(p: Path<Node>, exclusion: set<Node>)
+    {
+        forall i: nat :: i < |p.v| ==> p.v[i] !in exclusion
+    }
+
+    lemma NodeInExclusionNotInPath<Node>(p: Path<Node>, exclusion: set<Node>, n: Node)
+        requires PathExcludes(p, exclusion)
+        requires n in exclusion
+        ensures n !in p.v
+    {
+        reveal PathExcludes();
+    }
+
+    predicate NextNode<Node>(g: Digraph, n: Node, m: Node)
+        requires DigraphValid(g)
+        requires g.IsNode(n)
+    {
+        g.IsNode(m) && g.IsConnected(n, m)
+    }
+
+    function PathPrepend<Node>(g: Digraph, p: Path<Node>, n: Node): (r: Path<Node>)
+        // Add a node onto a path.
+        requires g.IsNode(n)
+        requires |p.v| > 0
+        requires g.IsConnected(n, p.v[0])
+        requires PathValid(g, p)
+        ensures PathValid(g, r)
+    {
+        reveal PathValid();
+        Path([n] + p.v)
+    }
+
+    lemma PathPrependNoRepeats<Node>(g: Digraph, p: Path<Node>, n: Node)
+        requires g.IsNode(n)
+        requires |p.v| > 0
+        requires g.IsConnected(n, p.v[0])
+        requires PathValid(g, p)
+        requires PathNoRepeats(p)
+        requires n !in p.v
+        ensures
+            var r := PathPrepend(g, p, n);
+            PathNoRepeats(r)
+    {
+    }
+
+    lemma PathPrependExcludes<Node>(
+            g: Digraph, p: Path<Node>, n: Node, exclusion: set<Node>)
+        requires g.IsNode(n)
+        requires |p.v| > 0
+        requires g.IsConnected(n, p.v[0])
+        requires PathValid(g, p)
+        requires PathExcludes(p, exclusion)
+        requires n !in exclusion
+        ensures
+            var r := PathPrepend(g, p, n);
+            PathExcludes(r, exclusion)
+    {
+        reveal PathExcludes();
+    }
+
+    lemma PathAppendOneBigger<Node>(g: Digraph, p: Path<Node>, n: Node)
+        // If we add a node to a path that wasn't already in it
+        // then that path contains one more node.
+        requires g.IsNode(n)
+        requires |p.v| > 0
+        requires g.IsConnected(PathEnd(p), n)
+        requires PathValid(g, p)
+        requires n !in p.v
+        ensures
+            var q := PathAppend(g, p, n);
+            |PathSet(p)| + 1 == |PathSet(q)|
+    {
+        reveal Seq.ToSet();
+        var q := PathAppend(g, p, n);
+        assert q.v == p.v + [n];
+        SeqExt.LemmaToSetAdds(p.v, [n]);
+        assert Seq.ToSet(p.v) + Seq.ToSet([n]) == Seq.ToSet(q.v);
+        assert PathSet(p) + {n} == PathSet(q);
+    }
+    
+    function RemovePathEnd<Node>(p: Path<Node>): Path<Node>
+        requires |p.v| > 0
+    {
+        Path(p.v[..|p.v|-1])
+    }
+
+    lemma IfNoRepeatsEndNotinRemovePathEnd<Node>(p: Path<Node>)
+        requires PathNoRepeats(p)
+        requires |p.v| > 0
+        ensures PathEnd(p) !in RemovePathEnd(p).v
+    {
+    }
+
+    lemma RemoveLoopsNoRepeats<Node>(p: Path<Node>)
+        requires |p.v| > 1
+        ensures
+            var q := PathRemoveLoopsInternal(p, |p.v|-1);
+            PathNoRepeats(q)
+    {
+        RemoveLoopsNoRepeatsInternal(p, |p.v|-1);
+    }
+
+    lemma RemoveLoopsNoRepeatsInternal<Node>(p: Path<Node>, index: nat)
+        requires index < |p.v|
+        ensures
+            var q := PathRemoveLoopsInternal(p, index);
+            PathNoRepeats(q)
+    {
+        var q := PathRemoveLoopsInternal(p, index);
+        if index == 0 {
+            var q := Path([p.v[0]]);
+            assert |q.v| == 1;
+            assert PathNoRepeats(q);
+        } else { 
+            var earlier_path := PathRemoveLoopsInternal(p, index-1);
+            var n := p.v[index];
+            if n in earlier_path.v {
+                var loc := PathFindIndex(earlier_path, n);
+                var q := Path(earlier_path.v[0..loc+1]);
+                assert PathNoRepeats(q);
+            } else {
+                var q := Path(earlier_path.v + [n]);
+                assert PathNoRepeats(q);
+            }
+        }
+    }
+
+    ghost predicate SimplePathExists<Node(!new)>(g: Digraph, a: Node, b: Node)
+    {
+        exists p: Path<Node> :: SimplePathFromTo(g, p, a, b)
+    }
+
+    ghost predicate SimpleShortExcludedPathExists<Node(!new)>(
+        g: Digraph, a: Node, b: Node, exclusion: set<Node>)
+    {
+        exists p: Path<Node> :: SimpleShortExcludedPathFromTo(g, p, a, b, exclusion)
+    }
+
+    lemma SimpleShortExcludedPathExistsByExample<Node>(
+        g: Digraph, p: Path<Node>, a: Node, b: Node, exclusion: set<Node>)
+        requires SimpleShortExcludedPathFromTo(g, p, a, b, exclusion)
+        ensures SimpleShortExcludedPathExists(g, a, b, exclusion)
+    {
+    }
+
+
+    lemma MaxPathLength<Node>(g: Digraph, p: Path<Node>)
+        requires PathNoRepeats(p)
+    {
+    }
+
+
+    function OneNodePath<Node>(g: Digraph, n: Node): (r: Path<Node>)
+        requires DigraphValid(g)
+        requires g.IsNode(n)
+        ensures PathValid(g, r)
+    {
+        reveal PathValid();
+        Path([n])
+    }
+
+    lemma NumberOfRemainingNodesDecreasesPath<Node>(g: Digraph, p: Path<Node>, n: Node)
+        requires DigraphValid(g)
+        requires PathValid(g, p)
+        requires PathNoRepeats(p)
+        requires NodeValid(g, n)
+        requires g.IsNode(n)
+        requires |p.v| > 0 ==> g.IsConnected(PathEnd(p), n)
+        requires n !in p.v
+        ensures
+            var new_p := PathAppend(g, p, n);
+            NumberOfRemainingNodesPath(g, new_p) <
+            NumberOfRemainingNodesPath(g, p)
+    {
+    }
+
+    lemma PathSetValid<Node>(g: Digraph, p: Path<Node>)
+        // If a path is valid, the nodes in it are valid.
+        requires DigraphValid(g)
+        requires PathValid(g, p)
+        ensures
+            var r := PathSet(p);
+            (forall n: Node :: n in r ==> NodeValid(g, n)) &&
+            (forall n: Node :: n in r ==> g.IsNode(n))
+    {
+        reveal Seq.ToSet();
+        reveal PathValid();
+        reveal DigraphValid();
+    }
+
+    function PathSetV<Node>(g: Digraph, p: Path<Node>): (r: set<Node>)
+        // A helper that combines the PathSet function and PathSetValid lemma.
+        // (I'm not sure if this is a sensible way of doing things, but it
+        //  feels like it helps us choose how many constraints we're instroducing).
+        requires DigraphValid(g)
+        requires PathValid(g, p)
+        ensures forall n: Node :: n in r ==> NodeValid(g, n)
+        ensures forall n: Node :: n in r ==> g.IsNode(n)
+    {
+        PathSetValid(g, p);
+        PathSet(p)
+    }
+
+    ghost predicate PathExistsR<Node(!new)>(g: Digraph, a: Node, b: Node)
+        // A Path Exists from a to b.
+        // A non-ghost version of SimplePathExists.
+        requires DigraphValid(g)
+        requires g.IsNode(a)
+        requires g.IsNode(b)
+    {
+        !PathDoesNotExistRecursiveInternal(g, a, b, {})
+    }
+
+    ghost predicate PathDoesNotExistRecursiveInternal<Node(!new)>(
+            g: Digraph, a: Node, b: Node, visited_nodes: set<Node>)
+        requires DigraphValid(g)
+        requires a !in visited_nodes
+        requires b !in visited_nodes
+        requires forall n :: n in visited_nodes ==> g.IsNode(n)
+        requires g.IsNode(a)
+        requires g.IsNode(b)
+        decreases NumberOfRemainingNodes(g, visited_nodes)
+    {
+        var new_visited_nodes := visited_nodes + {a};
+        assert |new_visited_nodes| == |visited_nodes| + 1;
+        if (a == b) then
+            false
+        else
+            forall n: Node :: (NextNode(g, a, n) && g.NodeMap(n) < g.NodeBound &&
+                n !in new_visited_nodes) ==>
+                    PathDoesNotExistRecursiveInternal(g, n, b, new_visited_nodes)
+    }
+
+    lemma {:vcs_split_on_every_assert} NotPathExistsIsPathDoesNotExistRecursive<Node(!new)>(
+            g: Digraph, b: Node, p: Path<Node>)
+        requires DigraphValid(g)
+        requires |p.v| > 0
+        requires b !in PathSet(RemovePathEnd(p))
+        requires PathValid(g, p)
+        requires PathNoRepeats(p)
+        requires g.IsNode(b)
+        decreases
+            reveal Seq.ToSet();
+            reveal PathValid();
+            NumberOfRemainingNodes(g, PathSet(p))
+        ensures
+            var visited_nodes := PathSet(RemovePathEnd(p));
+            var end := PathEnd(p);
+            reveal Seq.ToSet();
+            !SimpleShortExcludedPathExists(g, end, b, visited_nodes) ==
+                PathDoesNotExistRecursiveInternal(g, PathEnd(p), b, visited_nodes)
+    {
+        var visited_nodes := PathSet(RemovePathEnd(p));
+        var new_visited_nodes := PathSet(p);
+        var end := PathEnd(p);
+        reveal PathValid();
+        assert g.IsNode(end);
+        reveal Seq.ToSet();
+        assert new_visited_nodes == visited_nodes + {end};
+        assert |new_visited_nodes| == |visited_nodes| + 1;
+        assert |PathSet(p)| > |PathSet(RemovePathEnd(p))|;
+        assert end !in visited_nodes;
+        if (end == b) {
+            reveal PathValid();
+            assert !PathDoesNotExistRecursiveInternal(
+                g, end, b, visited_nodes);
+            var esp := Path([end]);
+            reveal PathExcludes();
+            SimpleShortExcludedPathExistsByExample(
+                g, esp, end, b, visited_nodes);
+            assert SimpleShortExcludedPathExists(g, end, b, visited_nodes);
+            assert !SimpleShortExcludedPathExists(g, end, b, visited_nodes) ==
+                PathDoesNotExistRecursiveInternal(g, PathEnd(p), b, visited_nodes);
+        } else {
+            // Show that if of the children has a path
+            // then this has a path.
+            // Show that otherwise then this does not have a path.
+            if exists n: Node :: NextNode(g, end, n) && g.NodeMap(n) < g.NodeBound &&
+                    n !in new_visited_nodes &&
+                    SimpleShortExcludedPathExists(g, n, b, new_visited_nodes) {
+                var n: Node :| NextNode(g, end, n) && g.NodeMap(n) < g.NodeBound &&
+                    n !in new_visited_nodes &&
+                    SimpleShortExcludedPathExists(g, n, b, new_visited_nodes);
+                assert SimpleShortExcludedPathExists(g, n, b, new_visited_nodes);  
+                var shorter: Path<Node> :| SimpleShortExcludedPathFromTo(
+                    g, shorter, n, b, new_visited_nodes);
+                reveal PathExcludes();
+                PathPrependNoRepeats(g, shorter, end);
+                PathPrependExcludes(g, shorter, end, visited_nodes);
+                var longer: Path<Node> := PathPrepend(g, shorter, end);
+                SimpleShortExcludedPathExistsByExample(
+                    g, longer, end, b, visited_nodes);
+                assert SimpleShortExcludedPathExists(g, end, b, visited_nodes);
+                var new_path := PathAppend(g, p, n);
+                NumberOfRemainingNodesDecreases(g, PathSet(p), n, PathSet(new_path));
+                NotPathExistsIsPathDoesNotExistRecursive(g, b, new_path);
+                assert !PathDoesNotExistRecursiveInternal(
+                    g, PathEnd(new_path), b, new_visited_nodes);
+                assert !PathDoesNotExistRecursiveInternal(g, PathEnd(p), b, visited_nodes);
+            } else {
+                if SimpleShortExcludedPathExists(g, end, b, visited_nodes) {
+                    var sse: Path<Node> :| SimpleShortExcludedPathFromTo(
+                        g, sse, end, b, visited_nodes);
+                    var n := sse.v[1];
+                    assert NextNode(g, end, n);
+                    reveal PathValid();
+                    ValidNodeBound(g, n);
+                    assert g.NodeMap(n) < g.NodeBound;
+                    reveal PathExcludes();
+                    assert n !in new_visited_nodes;
+                    var shorter := Path(sse.v[1..]);
+                    SimpleShortExcludedPathExistsByExample(
+                        g, shorter, n, b, new_visited_nodes);
+                    assert SimpleShortExcludedPathExists(g, n, b, new_visited_nodes);
+                    // This constradicts that such as 'n' does not exist.
+                    assert false;
+                }
+                forall n: Node | NextNode(g, end, n) && g.NodeMap(n) < g.NodeBound &&
+                        n !in new_visited_nodes
+                    ensures
+                        var new_path := PathAppend(g, p, n);
+                        PathDoesNotExistRecursiveInternal(g, n, b, new_visited_nodes)
+                {
+                    assert !SimpleShortExcludedPathExists(g, n, b, new_visited_nodes);
+                    var new_path := PathAppend(g, p, n);
+                    NumberOfRemainingNodesDecreases(g, PathSet(p), n, PathSet(new_path));
+                    NotPathExistsIsPathDoesNotExistRecursive(g, b, new_path);
+                    assert PathDoesNotExistRecursiveInternal(g, n, b, new_visited_nodes);
+                }
+                assert !SimpleShortExcludedPathExists(g, end, b, visited_nodes);
+                assert PathDoesNotExistRecursiveInternal(g, end, b, visited_nodes);
+            }
+        }
+    }
+
+    predicate SimplePathFromTo<Node(==)>(g: Digraph, p: Path<Node>, a: Node, b: Node)
+        // That path is valid and has no repeats (except possibly the end points).
+    {
+        PathValid(g, p) && |p.v| > 1 && (p.v[0] == a) && (p.v[|p.v|-1] == b) &&
+        PathNoRepeats(Path(p.v[0..|p.v|-2]))
+    }
+
+    predicate SimpleShortExcludedPathFromTo<Node>(
+        g: Digraph, p: Path<Node>, a: Node, b: Node, exclusion: set<Node>)
+        // That path is valid and has no repeats
+        // and doesn't go through any nodes in exclusion
+    {
+        PathValid(g, p) && |p.v| > 0 && (p.v[0] == a) && (p.v[|p.v|-1] == b) &&
+        PathNoRepeats(p) &&
+        PathExcludes(p, exclusion)
+    }
+
+    lemma NotNodePathInvalid<Node>(g: Digraph, n: Node, p: Path<Node>)
+        requires !g.IsNode(n)
+        requires n in p.v
+        ensures !PathValid(g, p)
+    {
+        reveal PathValid();
+    }
+
+
+    lemma IsNodeImpliesNodeValid<Node>(g: Digraph, n: Node)
+        requires DigraphValid(g)
+        requires g.IsNode(n)
+        ensures NodeValid(g, n)
+    {
+        reveal DigraphValid();
+    }
+
+
+}
