Digraph/DigraphPaths.dfy
@@ -1,0 +1,393 @@
+module DigraphPaths {
+
+    import Std.Collections.Seq
+
+    import Utils
+    import opened DigraphBase
+
+    ghost predicate {:opaque} DigraphLoop<Node(!new)>(g: Digraph)
+        // There's a loop in the digraph.
+        // (there exists a path that is a loop).
+    {
+        exists p: Path<Node> :: PathValid(g, p) && PathLoop(p)
+    }
+
+    ghost predicate {:opaque} DigraphLoop2<Node(!new)>(g: Digraph)
+        // There's a loop in the digraph.
+        // (there exists a node which has a path goes to itself)
+    {
+        exists n: Node :: PathExists(g, n, n)
+    }
+
+    lemma PathExistsToDigraphLoop2<Node>(g: Digraph, n: Node)
+        requires PathExists(g, n, n)
+        ensures DigraphLoop2(g)
+    {
+        reveal DigraphLoop2();
+    }
+
+    lemma DigraphLoopEquiv<Node(!new)>(g: Digraph)
+        // The two definitions for whether the digraph has a loop
+        // are equivalent.
+        ensures DigraphLoop(g) == DigraphLoop2(g)
+    {
+        reveal DigraphLoop();
+        reveal DigraphLoop2();
+        if DigraphLoop(g) {
+            var p :| PathValid(g, p) && PathLoop(p);
+            assert PathFromTo(g, p, p.v[0], p.v[0]);
+            assert PathExists(g, p.v[0], p.v[0]);
+            PathExistsToDigraphLoop2(g, p.v[0]);
+            assert DigraphLoop2(g);
+        } else {
+        }
+    }
+
+    ghost function GetLoopPath<Node(!new)>(g: Digraph): (r: Path<Node>)
+        // Returns a loop from a digraph that has a loop.
+        requires DigraphLoop(g)
+    {
+        reveal DigraphLoop();
+        DigraphLoopEquiv(g);
+        assert DigraphLoop2(g);
+        reveal DigraphLoop2();
+        var n :| PathExists(g, n, n);
+        var p :| PathValid(g, p) && |p.v| > 1 && p.v[0] == n && p.v[|p.v|-1] == n;
+        p
+    }
+
+    predicate PathLoop<Node(==)>(p: Path<Node>)
+        // The path starts and stop at the same place.
+    {
+        |p.v| > 1 && p.v[0] == p.v[|p.v|-1]
+    }
+
+    predicate PathNoRepeats<Node(==)>(p: Path<Node>)
+        // This path does not contain any repeated nodes.
+    {
+        forall i: nat, j: nat :: i < |p.v| && j < |p.v| && i != j ==> p.v[i] != p.v[j]
+    }
+
+    lemma NoLoopsMeansNoRepeats<Node(!new)>(g: Digraph<Node>)
+        requires !DigraphLoop(g)
+        ensures !exists p: Path<Node> :: PathValid(g, p) && !PathNoRepeats(p)
+    {
+        if exists p: Path<Node> :: PathValid(g, p) && !PathNoRepeats(p) {
+            var p : Path<Node> :| PathValid(g, p) && !PathNoRepeats(p);
+            assert PathValid(g, p);
+            var i: nat, j: nat :| (i < |p.v|) && (j < |p.v|) && (j > i) && (p.v[i] == p.v[j]);
+            var p_loop := PathSegment(p, i, j+1);
+            PathSegmentValid(g, p, i, j+1);
+            assert PathValid(g, p_loop);
+            assert PathLoop(p_loop);
+            reveal DigraphLoop();
+            assert DigraphLoop(g);
+            assert false;
+        }
+    }
+
+    lemma NoRepeatsIsHasNoDuplicates<Node>(p: Path<Node>)
+        requires PathNoRepeats(p)
+        ensures Seq.HasNoDuplicates(p.v)
+    {
+        reveal Seq.HasNoDuplicates();
+    }
+
+    predicate PathSimpleLoop<Node(==)>(p: Path<Node>)
+        // A simple loop is a loop which doesn't have any repeats
+        // (apart from the start and stop)
+    {
+        PathLoop(p) && PathNoRepeats(Path(p.v[1..|p.v|]))
+    }
+
+    ghost predicate PathExists<Node(!new)>(g: Digraph, a: Node, b: Node)
+    {
+        exists p: Path<Node> :: PathFromTo(g, p, a, b)
+    }
+
+    predicate PathFromTo<Node(==)>(g: Digraph, p: Path<Node>, a: Node, b: Node)
+        // The path is valid and goes between these parts.
+    {
+        PathValid(g, p) && |p.v| > 1 && (p.v[0] == a) && (p.v[|p.v|-1] == b)
+    }
+
+    function PathSegment<Node>(p: Path<Node>, start: nat, stop: nat): (r: Path<Node>)
+        // Create a new path by taking a segment of an existing one.
+        requires start < |p.v|
+        requires stop <= |p.v|
+        requires start < stop
+        ensures |r.v| > 0
+    {
+        Path(p.v[start..stop])
+    }
+
+    lemma PathSegmentValid<Node>(g: Digraph, p: Path<Node>, start: nat, stop: nat)
+        // A segment of a valid path is a valid path.
+        requires start < |p.v|
+        requires stop <= |p.v|
+        requires start < stop
+        requires PathValid(g, p)
+        ensures 
+            var r := PathSegment(p, start, stop);
+            PathValid(g, r)
+    {
+        reveal PathValid();
+    }
+
+    lemma PathExistsByExample<Node>(g: Digraph, p: Path<Node>, a: Node, b: Node)
+        requires PathFromTo(g, p, a, b)
+        ensures PathExists(g, a, b)
+    {
+    }
+
+    function PathFindIndexInternal<Node(==)>(p: Path<Node>, n: Node, index: nat): (r: nat)
+        requires index < |p.v|
+        requires n in p.v[index..|p.v|]
+        ensures r < |p.v|
+        ensures p.v[r] == n
+        decreases |p.v| - index
+    {
+        if p.v[index] == n then
+            index
+        else
+            PathFindIndexInternal(p, n, index+1)
+    }
+
+    function PathFindIndex<Node(==)>(p: Path<Node>, n: Node): (r: nat)
+        // Find the position of a node in a path. 
+        requires n in p.v
+        ensures r < |p.v|
+        ensures p.v[r] == n
+    {
+        PathFindIndexInternal(p, n, 0)
+    }
+
+    lemma PathExistsAdd<Node(!new)>(g: Digraph, a: Node, b: Node, c: Node)
+        requires PathExists(g, a, b)
+        requires PathExists(g, b, c)
+        ensures PathExists(g, a, c)
+    {
+        var p :| PathFromTo(g, p, a, b);
+        var q :| PathFromTo(g, q, b, c);
+        assert |q.v| > 1;
+        var pq := Path(p.v[0..|p.v|] + q.v[1..|q.v|]);
+        reveal PathValid();
+        assert PathValid(g, pq);
+        assert PathFromTo(g, pq, a, c);
+    }
+
+    function NumberOfRemainingNodes<Node>(g: Digraph, visited_nodes: set<Node>): nat
+        // This is useful when we want to show that something that walks the
+        // graph will terminate.
+        requires DigraphValid(g)
+        requires forall n :: n in visited_nodes ==> g.IsNode(n)
+    {
+        NodeSetSize(g, visited_nodes);
+        g.NodeBound - |visited_nodes|
+    }
+
+    function NumberOfRemainingNodesPath<Node(==)>(g: Digraph, p: Path<Node>): nat
+        // This is useful when we want to show that something that walks the
+        // graph will terminate.
+        requires DigraphValid(g)
+        requires PathValid(g, p)
+        requires PathNoRepeats(p)
+    {
+        NoRepeatsPathSetSize(p);
+        var s := PathSet(p);
+        assert forall x :: x in s ==> x in p.v;
+        reveal PathValid();
+        assert forall x :: x in p.v ==> g.IsNode(x);
+        NodeSetSize(g, s);
+        assert |p.v| <= g.NodeBound;
+        g.NodeBound - |p.v|
+    }
+
+    lemma NumberOfRemainingNodesDecreases<Node>(
+        g: Digraph, visited_nodes: set<Node>, n: Node, new_visited_nodes: set<Node>)
+        requires DigraphValid(g)
+        requires forall m :: m in visited_nodes ==> g.IsNode(m)
+        requires g.IsNode(n)
+        requires n !in visited_nodes
+        requires new_visited_nodes == visited_nodes + {n}
+        ensures
+            NumberOfRemainingNodes(g, new_visited_nodes) <
+            NumberOfRemainingNodes(g, visited_nodes)
+    {
+    }
+
+    lemma NodeSetSize<Node>(g: Digraph, nodes: set<Node>)
+        // Lets us set an upper bound on the number of nodes in a graph.
+        requires DigraphValid(g)
+        requires forall n: Node :: n in nodes ==> g.IsNode(n)
+        ensures |nodes| <= g.NodeBound
+    {
+        reveal DigraphValid();
+        assert forall n: Node :: n in nodes ==> g.NodeMap(n) < g.NodeBound;
+        var f := (n: Node) => g.NodeMap(n);
+        var nodes_as_nats := set n | n in nodes :: f(n);
+        Utils.MappedSetSize(nodes, f, nodes_as_nats);
+        assert |nodes_as_nats| == |nodes|;
+        Utils.BoundedSetSize(g.NodeBound as nat, nodes_as_nats);
+    }
+
+    lemma NoRepeatsPathSetSize<Node>(p: Path<Node>)
+        requires PathNoRepeats(p)
+        ensures |PathSet(p)| == |p.v|
+    {
+        NoRepeatsIsHasNoDuplicates(p);
+        Seq.LemmaCardinalityOfSetNoDuplicates(p.v);
+    }
+
+    function PathSet<Node>(p: Path<Node>): (r: set<Node>)
+        ensures forall x :: x in r ==> x in p.v
+    {
+        reveal Seq.ToSet();
+        Seq.ToSet(p.v)
+    }
+
+    function PathEnd<Node>(p: Path<Node>): Node
+        requires |p.v| > 0
+    {
+        p.v[|p.v|-1]
+    }
+
+    function PathStart<Node>(p: Path<Node>): Node
+        requires |p.v| > 0
+    {
+        p.v[0]
+    }
+
+    function AddPaths<Node>(p1: Path<Node>, p2: Path<Node>): (r: Path<Node>)
+        requires |p1.v| > 0
+        requires |p2.v| > 0
+        requires p1.v[|p1.v|-1] == p2.v[0]
+    {
+        var p2t := if |p2.v| > 1 then p2.v[1..|p2.v|] else [];
+        Path(p1.v + p2t)
+    }
+
+    lemma AddPathsValid<Node>(g: Digraph, p1: Path<Node>, p2: Path<Node>)
+        requires PathValid(g, p1)
+        requires PathValid(g, p2)
+        requires |p1.v| > 0
+        requires |p2.v| > 0
+        requires p1.v[|p1.v|-1] == p2.v[0]
+        ensures
+            var r := AddPaths(p1, p2);
+            PathValid(g, r)
+    {
+        reveal PathValid();
+    }
+
+    function PathAppend<Node>(g: Digraph, p: Path<Node>, n: Node): (r: Path<Node>)
+        // Add a node onto a path.
+        requires g.IsNode(n)
+        requires |p.v| > 0 ==> g.IsConnected(p.v[|p.v|-1], n)
+        requires PathValid(g, p)
+        ensures PathValid(g, r)
+    {
+        reveal PathValid();
+        Path(p.v + [n])
+    }
+
+    lemma AddPathsFromTo<Node>(g: Digraph, p1: Path<Node>, p2: Path<Node>)
+        requires PathValid(g, p1)
+        requires PathValid(g, p2)
+        requires |p1.v| > 0
+        requires |p2.v| > 0
+        requires PathEnd(p1) == PathStart(p2)
+        ensures
+            var r := AddPaths(p1, p2);
+            var a := PathStart(p1);
+            var c := PathEnd(p2);
+            ShortPathFromTo(g, r, a, c) &&
+            |r.v| == |p1.v| + |p2.v| - 1
+    {
+        AddPathsValid(g, p1, p2);
+    }
+
+    predicate ShortPathFromTo<Node(==)>(g: Digraph, p: Path<Node>, a: Node, b: Node)
+        // A valid path between two ports.  But a path of length 1 is allowed.
+    {
+        PathValid(g, p) && |p.v| > 0 && (p.v[0] == a) && (p.v[|p.v|-1] == b)
+    }
+    
+    function PathRemoveLoops<Node(==)>(p: Path<Node>): (r: Path<Node>)
+        // Creates a new path by snipping off any loops that
+        // exist in the path.
+        requires |p.v| > 0
+    {
+        PathRemoveLoopsInternal(p, |p.v|-1)
+    }
+
+    function PathRemoveLoopsInternal<Node(==)>(p: Path<Node>, index: nat): (r: Path<Node>)
+        requires index < |p.v|
+        decreases index
+    {
+        if index == 0 then
+            Path([p.v[0]])
+        else 
+            var earlier_path := PathRemoveLoopsInternal(p, index-1);
+            var n := p.v[index];
+            if n in earlier_path.v then
+                var loc := PathFindIndex(earlier_path, n);
+                Path(earlier_path.v[0..loc+1])
+            else
+                Path(earlier_path.v + [n])
+    }
+
+    lemma RemoveLoopsFromToSame<Node>(g: Digraph, p: Path<Node>)
+        // When we remove loops we get a path with the same
+        // start and end.  Possibly of length 1 node.
+        // It won't have repeats.
+        requires |p.v| > 1
+        requires p.v[0] != p.v[|p.v|-1]
+        requires PathValid(g, p)
+        ensures
+            var a := p.v[0];
+            var b := p.v[|p.v|-1];
+            var q := PathRemoveLoops(p);
+            ShortPathFromTo(g, q, a, b) &&
+            PathNoRepeats(q)
+    {
+        RemoveLoopsFromToSameInternal(g, p, |p.v|-1);
+    }
+
+    lemma RemoveLoopsFromToSameInternal<Node>(g: Digraph, p: Path<Node>, index: nat)
+        requires index < |p.v|
+        requires |p.v| > 1
+        requires p.v[0] != p.v[|p.v|-1]
+        requires PathValid(g, p)
+        ensures
+            var a := p.v[0];
+            var b := p.v[index];
+            var q := PathRemoveLoopsInternal(p, index);
+            ShortPathFromTo(g, q, a, b) &&
+            PathNoRepeats(q)
+    {
+        var a := p.v[0];
+        var b := p.v[index];
+        var q := PathRemoveLoopsInternal(p, index);
+        if index == 0 {
+            assert q == Path([a]);
+            reveal PathValid();
+            assert ShortPathFromTo(g, q, a, b);
+        } else {
+            var earlier_path := PathRemoveLoopsInternal(p, index-1);
+            RemoveLoopsFromToSameInternal(g, p, index-1);
+            var n := p.v[index];
+            if n in earlier_path.v {
+                var loc := PathFindIndex(earlier_path, n);
+                assert q == Path(earlier_path.v[0..loc+1]);
+            } else {
+                assert q == Path(earlier_path.v + [n]);
+            }
+            reveal PathValid();
+            assert PathValid(g, earlier_path);
+            assert PathValid(g, q);
+            assert ShortPathFromTo(g, q, a, b);
+        }
+    }
+
+}
