Test/CircuitTest.dfy
@@ -1,0 +1,120 @@
+module CircuitTest {
+
+    import opened Std.Wrappers
+    import opened Primitives
+    import Std.Collections.Map
+    import opened CircuitBase
+    import opened CircuitEvaluate
+    import opened CircuitHPNP
+    import opened CircuitHierarchy
+    import opened CircuitToGraph
+    import opened CircuitBuild
+    import DG = DigraphBase
+    import P = Primitives
+    // Make a circuit with a single XOR gate.
+
+    const i0_n: CNode := 0
+    const i1_n: CNode := 1
+    const o_n: CNode := 2
+    const xor_n: CNode := 3
+
+    const i0_p := NP(i0_n, OUTPUT_PORT)
+    const i1_p := NP(i1_n, OUTPUT_PORT)
+    const o_p := NP(o_n, INPUT_PORT)
+
+    const xor_i0 := NP(xor_n, 0)
+    const xor_i1 := NP(xor_n, 1)
+    const xor_o := NP(xor_n, 2)
+
+    const circ := Circuit(
+        NodeKind := (n: CNode) => (match n
+            case i0_n => Some(CInput())
+            case i1_n => Some(CInput())
+            case o_n => Some(COutput())
+            case xor_n => Some(nk_xor)
+            case _ => None
+            ),
+        PortSource := (np: NP) => (match np
+            case NP(3, 0) => Some(i0_p)
+            case NP(3, 1) => Some(i1_p)
+            case NP(2, 0) => Some(xor_o)
+            case _ => None),
+        PortNames := _ => None,
+        NodeBound := 4,
+        PortBound := 3,
+        HierLevel := 0
+    )
+    const HierLevel: nat := 0
+    const PortBound: CPort := 4
+
+    lemma Stuff()
+    {
+        CircValid();
+        assert NPValid(circ, xor_i0);
+        var xor_i0_hpnp := HPNP(HPNode(HP([]), xor_n), 0);
+        reveal HPNPValidInput();
+        reveal HPNPValidOutput();
+        assert HPNPValid(circ, xor_i0_hpnp);
+    }
+
+    lemma CircValid()
+        ensures CircuitValid(circ)
+    {
+        reveal CircuitValid();
+    }
+
+    lemma CircComplete()
+        ensures CircuitValid(circ)
+        ensures CircuitComplete(circ)
+    {
+        CircValid();
+        reveal CircuitComplete();
+    }
+
+    lemma CircNoLoops()
+        ensures CircuitValid(circ)
+        ensures CircuitComplete(circ)
+        ensures CircuitNoLoops(circ)
+    {
+        CircValid();
+        CircComplete();
+        var g := CtoGV(circ);
+        var all_nodes := DG.AllNodes(g);
+        assert |all_nodes| == 6;
+    }
+
+    lemma Blah()
+    {
+        var c := circ;
+        var i0 := HPNP(HPNode(HP([]), 0), OUTPUT_PORT);
+        var i1 := HPNP(HPNode(HP([]), 1), OUTPUT_PORT);
+        var o := HPNP(HPNode(HP([]), 2), INPUT_PORT);
+        var isigs: HPNP -> bool := (hpnp: HPNP) =>
+            if hpnp == i0 then true
+            else if hpnp == i0 then true
+            else false;
+        CircValid();
+        CircComplete();
+        CircNoLoops();
+        var b := EvaluateONP(c, isigs, DG.Path([]));
+    }
+
+    function MakeOneBitAdder(): Circuit
+    {
+        var g := MakeEmptyCircuit();
+        assert CircuitValid(g);
+        var (g, i_0) := AddIPort(g);
+        assert CircuitValid(g);
+        var (g, i_1) := AddIPort(g);
+        var (g, node_xor) := AddNode(g, P.nk_xor, map[0 := i_0, 1 := i_1]);
+        var xor_output := NP(node_xor, 0);
+        var g := AddOPort(g, xor_output);
+        var (g, node_add) := AddNode(g, P.nk_and, map[0 := i_0, 1 := i_1]);
+        var add_output := NP(node_add, 0);
+        var g := AddOPort(g, add_output);
+        assert CircuitValid(g);
+        g
+    }
+
+
+}
