Utils/SetExt.dfy
@@ -1,0 +1,14 @@
+module SetExt {
+
+  ///* Returns the maximum integer value in a non-empty set of integers. */
+  //function {:opaque} Max(xs: set<int>): int
+  //  requires 0 < |xs|
+  //  ensures forall k :: k in xs ==> Max(xs) >= k
+  //  ensures Max(xs) in xs
+  //{
+  //  var y :| 
+  //  assert xs == [xs[0]] + xs[1..];
+  //  if |xs| == 1 then xs[0] else Math.Max(xs[0], Max(xs[1..]))
+  //}
+
+}
